An example closer to a real security policy

Examples.v
@@ -25,3 +25,51 @@ Module OnlyPositive.
     destruct v; refines.
   Qed.
 End OnlyPositive.
+
+
+Module Restriction.
+  Definition chs : channels := fun _ => nat.
+
+  Definition pr1 : process chs :=
+    #!chs["output", 1], #!chs["output", 2], Done.
+
+  CoFixpoint monitor : process chs :=
+    #?chs["intermediate", n],
+    match n with
+      | O => monitor
+      | _ => #!chs["output", n], monitor
+    end.
+
+  Theorem monitor_eq : monitor = #?chs["intermediate", n],
+                       match n with
+                         | O => monitor
+                         | _ => #!chs["output", n], monitor
+                       end.
+  Proof.
+    rewrite expand_ok at 1; auto.
+  Qed.
+
+  Definition pr2 (pr : process chs) : process chs :=
+    (##[(Send, "intermediate")], pr)
+    || monitor.
+
+  Lemma pr1_pr2' : forall n k pr, refines k (pr2 pr)
+    -> refines (#!chs["output", S n], k) (pr2 (#!chs["intermediate", S n], pr)).
+  Proof.
+    intros.
+    unfold pr2.
+    rewrite monitor_eq.
+    apply match_right_restricted.
+    simpl; tauto.
+    apply send_send.
+    auto.
+  Qed.    
+
+  Theorem pr1_pr2 : exists pr, refines pr1 (pr2 pr).
+  Proof.
+    eexists.
+    repeat apply pr1_pr2'.
+    instantiate (1 := Done).
+    refines.
+  Qed.
+End Restriction.
