Refinement.v
@@ -60,6 +60,79 @@ Section Refinement.
     eauto.
   Qed.
 
+  Lemma traceEqual_interleave : forall tr tr',
+    traceEqual (chs := chs) tr' tr
+    -> forall tr1 tr2, interleave tr1 tr2 tr
+    -> interleave tr1 tr2 tr'.
+  Proof.
+    cofix; destruct 2.
+
+    destruct H.
+    constructor.
+    econstructor; eauto.
+
+    destruct H.
+    constructor.
+    econstructor; eauto.
+
+    inv H.
+    eauto.
+
+    inv H.
+    eauto.
+
+    eauto.
+    eauto.
+  Qed.
+
+  Hint Immediate traceEqual_interleave.
+
+  Theorem recv_recv_restricted : forall (which : direction * channel -> Prop) ch k k' k'',
+    which (Recv, ch)
+    -> (forall v, refines (k v) (Restrict which (k' v) || k''))
+    -> refines (DoRecv (chs := chs) ch k) (Restrict which (DoRecv ch k') || k'').
+  Proof.
+    intros; hnf; intros.
+    inv H1; eauto.
+
+    apply H0 in H5; clear H0; firstorder.
+    inv H0.
+    Focus 2.
+
+    inv H1.
+    eexists; split.
+    econstructor.
+    econstructor.
+    econstructor.
+    econstructor.
+    eauto.
+    eauto.
+    eauto.
+    eauto.
+
+    inv H4.
+    Focus 2.
+    eexists; split.
+    econstructor.
+    econstructor.
+    econstructor.
+    econstructor.
+    eauto.
+    eauto.
+    2: eauto.
+    eauto.
+
+    eexists; split.
+    econstructor.
+    econstructor.
+    econstructor.
+    eauto.
+    eauto.
+    eauto.
+    econstructor; eauto.
+    eauto.
+  Qed.
+
   Theorem match_right : forall ch k k' k'' v,
     refines k (k' || k'' v)
     -> refines (chs := chs) k (DoSend ch v k' || DoRecv ch k'').
@@ -75,6 +148,111 @@ Section Refinement.
     econstructor.
     eauto.
     econstructor.
+    eauto.
+    eauto.
+    auto.
+  Qed.
+
+  Lemma interleave_nil1 : forall tr1 tr2,
+    interleave (chs := chs) SNil tr1 tr2
+    -> traceEqual tr1 tr2.
+  Proof.
+    cofix; inversion 1; subst; intros.
+    eauto.
+    eauto.
+    constructor; eauto.
+  Qed.
+
+  Lemma traceEqual_sym : forall tr1 tr2,
+    traceEqual (chs := chs) tr1 tr2
+    -> traceEqual tr2 tr1.
+  Proof.
+    cofix; destruct 1; econstructor; eauto.
+  Qed.
+
+  Lemma traceEqual_trans : forall tr1 tr2 tr3,
+    traceEqual (chs := chs) tr1 tr2
+    -> traceEqual tr2 tr3
+    -> traceEqual tr1 tr3.
+  Proof.
+    cofix; destruct 1; inversion 1; econstructor; eauto.
+  Qed.
+
+  Theorem match_right_restricted : forall (which : _ -> Prop) ch k k' k'' v,
+    which (Send, ch)
+    -> refines k (Restrict which k' || k'' v)
+    -> refines (chs := chs) k (Restrict which (DoSend ch v k') || DoRecv ch k'').
+  Proof.
+    intros; hnf; intros.
+    apply H0 in H1; clear H0; firstorder.
+    inv H0; subst.
+    Focus 2.
+    inv H1; eauto.
+
+    inv H4.
+    Focus 2.
+    apply interleave_nil1 in H7.
+    eexists; split.
+    econstructor.
+    econstructor.
+    econstructor.
+    eauto.
+    eauto.
+    econstructor.
+    eauto.
+    eauto.
+    eauto using traceEqual_trans, traceEqual_sym.
+
+    eexists; split.
+    econstructor.
+    econstructor.
+    econstructor.
+    eauto.
+    eauto.
+    econstructor; eauto.
+    eauto.
+    auto.
+  Qed.
+
+  Theorem send_send : forall ch k k' k'' v,
+    refines k (k' || k'')
+    -> refines (DoSend (chs := chs) ch v k) (k' || DoSend ch v k'').
+  Proof.
+    intros; hnf; intros.
+    inv H0; eauto.
+    apply H in H5; clear H; firstorder.
+    inv H.
+    Focus 2.
+
+    inv H0.
+    eexists; split.
+    econstructor.
+    eauto.
+    econstructor.
+    eauto.
+    eauto.
+    eauto.
+
+    eexists; split.
+    econstructor.
+    eauto.
+    econstructor.
+    eauto.
+    econstructor; eauto.
+    eauto.
+  Qed.
+
+  Theorem done_right_restricted : forall which k k',
+    refines k k'
+    -> refines (chs := chs) k (Restrict which Done || k').
+  Proof.
+    intros; hnf; intros.
+    apply H in H0; firstorder.
+    eexists; split.
+    econstructor.
+    econstructor.
+    eauto.
+    eauto.
     eauto.
     eauto.
     auto.
